% !TEX TS-program = XeLaTeX
\documentclass[varwidth=100cm]{standalone}
\usepackage{prooftree}

\begin{document}
For this tree we denote $s_{a,b}$ to denote $s[x->a][y->b]$.\\  

\begin{prooftree}
	\begin{prooftree}
		\begin{prooftree}
				\langle x := 0, s_{\bot,\bot} \rangle \rightarrow s_{0,\bot} \ ^{[ass_{ns}]}
				\langle y := 0, s_{0,\bot} \rangle \rightarrow s_{0,0} \ ^{[ass_{ns}]}
		\justifies
			\langle (x := 0; y := 0), s_{\bot,\bot}\rangle \rightarrow s_{0,0}
		\using
			[comp_{ns}]
		\end{prooftree}
		\begin{prooftree}
			\begin{prooftree}
					\langle x := (x + 1), s_{0,0} \rangle \rightarrow s_{1,0} \ ^{[ass_{ns}]}
					\langle y := (y + x), s_{1,0} \rangle \rightarrow s_{1,1} \ ^{[ass_{ns}]}
			\justifies
				\langle (x := (x + 1); y := (y + x)), s_{0,0}\rangle \rightarrow s_{1,1}
			\using
				[comp_{ns}]
			\end{prooftree}
			\begin{prooftree}
				\begin{prooftree}
						\langle x := (x + 1), s_{1,1} \rangle \rightarrow s_{2,1} \ ^{[ass_{ns}]}
						\langle y := (y + x), s_{2,1} \rangle \rightarrow s_{2,3} \ ^{[ass_{ns}]}
				\justifies
					\langle (x := (x + 1); y := (y + x)), s_{1,1}\rangle \rightarrow s_{2,3}
				\using
					[comp_{ns}]
				\end{prooftree}
				\begin{prooftree}
					\begin{prooftree}
							\langle x := (x + 1), s_{2,3} \rangle \rightarrow s_{3,3} \ ^{[ass_{ns}]}
							\langle y := (y + x), s_{3,3} \rangle \rightarrow s_{3,6} \ ^{[ass_{ns}]}
					\justifies
						\langle (x := (x + 1); y := (y + x)), s_{2,3}\rangle \rightarrow s_{3,6}
					\using
						[comp_{ns}]
					\end{prooftree}
						\langle $while $(x <= 2)$ do $(x := (x + 1); y := (y + x)), s_{3,6} \rangle \rightarrow s_{3,6} \ ^{[while_{ns}^{ff}]}
				\justifies
					\langle $while $(x <= 2)$ do $(x := (x + 1); y := (y + x)), s_{2,3}\rangle \rightarrow s_{3,6}
				\using
					[while_{ns}^{tt}]
				\end{prooftree}
			\justifies
				\langle $while $(x <= 2)$ do $(x := (x + 1); y := (y + x)), s_{1,1}\rangle \rightarrow s_{3,6}
			\using
				[while_{ns}^{tt}]
			\end{prooftree}
		\justifies
			\langle $while $(x <= 2)$ do $(x := (x + 1); y := (y + x)), s_{0,0}\rangle \rightarrow s_{3,6}
		\using
			[while_{ns}^{tt}]
		\end{prooftree}
	\justifies
		\langle ((x := 0; y := 0); $while $(x <= 2)$ do $(x := (x + 1); y := (y + x))), s_{\bot,\bot}\rangle \rightarrow s_{3,6}
	\using
		[comp_{ns}]
	\end{prooftree}
		\langle y := (2 * y), s_{3,6} \rangle \rightarrow s_{3,12} \ ^{[ass_{ns}]}
\justifies
	\langle (((x := 0; y := 0); $while $(x <= 2)$ do $(x := (x + 1); y := (y + x))); y := (2 * y)), s_{\bot,\bot}\rangle \rightarrow s_{3,12}
\using
	[comp_{ns}]
\end{prooftree}
\end{document}