% !TEX TS-program = XeLaTeX
\documentclass[varwidth=200cm]{standalone}
\usepackage{prooftree}
\usepackage{amsfonts} % for \mathbb{}

\begin{document}
For this tree we denote $s_{a,b}$ to denote $s[n->a][r->b]$, where $a,b\in \mathbb{N}$\\  

\begin{prooftree}
		\langle r := 1, s_{10,\bot} \rangle \rightarrow s_{10,1} \ ^{[ass_{ns}]}
	\begin{prooftree}
		\begin{prooftree}
				\langle r := r * n, s_{10,1} \rangle \rightarrow s_{10,10} \ ^{[ass_{ns}]}
				\langle n := n - 1, s_{10,10} \rangle \rightarrow s_{9,10} \ ^{[ass_{ns}]}
		\justifies
			\langle r := r * n; n := n - 1, s_{10,1}\rangle \rightarrow s_{9,10}
		\using
			[comp_{ns}]
		\end{prooftree}
		\begin{prooftree}
			\begin{prooftree}
					\langle r := r * n, s_{9,10} \rangle \rightarrow s_{9,90} \ ^{[ass_{ns}]}
					\langle n := n - 1, s_{9,90} \rangle \rightarrow s_{8,90} \ ^{[ass_{ns}]}
			\justifies
				\langle r := r * n; n := n - 1, s_{9,10}\rangle \rightarrow s_{8,90}
			\using
				[comp_{ns}]
			\end{prooftree}
			\begin{prooftree}
				\begin{prooftree}
						\langle r := r * n, s_{8,90} \rangle \rightarrow s_{8,720} \ ^{[ass_{ns}]}
						\langle n := n - 1, s_{8,720} \rangle \rightarrow s_{7,720} \ ^{[ass_{ns}]}
				\justifies
					\langle r := r * n; n := n - 1, s_{8,90}\rangle \rightarrow s_{7,720}
				\using
					[comp_{ns}]
				\end{prooftree}
				\begin{prooftree}
					\begin{prooftree}
							\langle r := r * n, s_{7,720} \rangle \rightarrow s_{7,5040} \ ^{[ass_{ns}]}
							\langle n := n - 1, s_{7,5040} \rangle \rightarrow s_{6,5040} \ ^{[ass_{ns}]}
					\justifies
						\langle r := r * n; n := n - 1, s_{7,720}\rangle \rightarrow s_{6,5040}
					\using
						[comp_{ns}]
					\end{prooftree}
					\begin{prooftree}
						\begin{prooftree}
								\langle r := r * n, s_{6,5040} \rangle \rightarrow s_{6,30240} \ ^{[ass_{ns}]}
								\langle n := n - 1, s_{6,30240} \rangle \rightarrow s_{5,30240} \ ^{[ass_{ns}]}
						\justifies
							\langle r := r * n; n := n - 1, s_{6,5040}\rangle \rightarrow s_{5,30240}
						\using
							[comp_{ns}]
						\end{prooftree}
						\begin{prooftree}
							\begin{prooftree}
									\langle r := r * n, s_{5,30240} \rangle \rightarrow s_{5,151200} \ ^{[ass_{ns}]}
									\langle n := n - 1, s_{5,151200} \rangle \rightarrow s_{4,151200} \ ^{[ass_{ns}]}
							\justifies
								\langle r := r * n; n := n - 1, s_{5,30240}\rangle \rightarrow s_{4,151200}
							\using
								[comp_{ns}]
							\end{prooftree}
							\begin{prooftree}
								\begin{prooftree}
										\langle r := r * n, s_{4,151200} \rangle \rightarrow s_{4,604800} \ ^{[ass_{ns}]}
										\langle n := n - 1, s_{4,604800} \rangle \rightarrow s_{3,604800} \ ^{[ass_{ns}]}
								\justifies
									\langle r := r * n; n := n - 1, s_{4,151200}\rangle \rightarrow s_{3,604800}
								\using
									[comp_{ns}]
								\end{prooftree}
								\begin{prooftree}
									\begin{prooftree}
											\langle r := r * n, s_{3,604800} \rangle \rightarrow s_{3,1814400} \ ^{[ass_{ns}]}
											\langle n := n - 1, s_{3,1814400} \rangle \rightarrow s_{2,1814400} \ ^{[ass_{ns}]}
									\justifies
										\langle r := r * n; n := n - 1, s_{3,604800}\rangle \rightarrow s_{2,1814400}
									\using
										[comp_{ns}]
									\end{prooftree}
									\begin{prooftree}
										\begin{prooftree}
												\langle r := r * n, s_{2,1814400} \rangle \rightarrow s_{2,3628800} \ ^{[ass_{ns}]}
												\langle n := n - 1, s_{2,3628800} \rangle \rightarrow s_{1,3628800} \ ^{[ass_{ns}]}
										\justifies
											\langle r := r * n; n := n - 1, s_{2,1814400}\rangle \rightarrow s_{1,3628800}
										\using
											[comp_{ns}]
										\end{prooftree}
										\begin{prooftree}
											\begin{prooftree}
													\langle r := r * n, s_{1,3628800} \rangle \rightarrow s_{1,3628800} \ ^{[ass_{ns}]}
													\langle n := n - 1, s_{1,3628800} \rangle \rightarrow s_{0,3628800} \ ^{[ass_{ns}]}
											\justifies
												\langle r := r * n; n := n - 1, s_{1,3628800}\rangle \rightarrow s_{0,3628800}
											\using
												[comp_{ns}]
											\end{prooftree}
												\langle $while $!n <= 0$ do $(r := r * n; n := n - 1), s_{0,3628800} \rangle \rightarrow s_{0,3628800} \ ^{[while_{ns}^{ff}]}
										\justifies
											\langle $while $!n <= 0$ do $(r := r * n; n := n - 1), s_{1,3628800}\rangle \rightarrow s_{0,3628800}
										\using
											[while_{ns}^{tt}]
										\end{prooftree}
									\justifies
										\langle $while $!n <= 0$ do $(r := r * n; n := n - 1), s_{2,1814400}\rangle \rightarrow s_{0,3628800}
									\using
										[while_{ns}^{tt}]
									\end{prooftree}
								\justifies
									\langle $while $!n <= 0$ do $(r := r * n; n := n - 1), s_{3,604800}\rangle \rightarrow s_{0,3628800}
								\using
									[while_{ns}^{tt}]
								\end{prooftree}
							\justifies
								\langle $while $!n <= 0$ do $(r := r * n; n := n - 1), s_{4,151200}\rangle \rightarrow s_{0,3628800}
							\using
								[while_{ns}^{tt}]
							\end{prooftree}
						\justifies
							\langle $while $!n <= 0$ do $(r := r * n; n := n - 1), s_{5,30240}\rangle \rightarrow s_{0,3628800}
						\using
							[while_{ns}^{tt}]
						\end{prooftree}
					\justifies
						\langle $while $!n <= 0$ do $(r := r * n; n := n - 1), s_{6,5040}\rangle \rightarrow s_{0,3628800}
					\using
						[while_{ns}^{tt}]
					\end{prooftree}
				\justifies
					\langle $while $!n <= 0$ do $(r := r * n; n := n - 1), s_{7,720}\rangle \rightarrow s_{0,3628800}
				\using
					[while_{ns}^{tt}]
				\end{prooftree}
			\justifies
				\langle $while $!n <= 0$ do $(r := r * n; n := n - 1), s_{8,90}\rangle \rightarrow s_{0,3628800}
			\using
				[while_{ns}^{tt}]
			\end{prooftree}
		\justifies
			\langle $while $!n <= 0$ do $(r := r * n; n := n - 1), s_{9,10}\rangle \rightarrow s_{0,3628800}
		\using
			[while_{ns}^{tt}]
		\end{prooftree}
	\justifies
		\langle $while $!n <= 0$ do $(r := r * n; n := n - 1), s_{10,1}\rangle \rightarrow s_{0,3628800}
	\using
		[while_{ns}^{tt}]
	\end{prooftree}
\justifies
	\langle r := 1; $while $!n <= 0$ do $(r := r * n; n := n - 1), s_{10,\bot}\rangle \rightarrow s_{0,3628800}
\using
	[comp_{ns}]
\end{prooftree}
\end{document}